src/SwitchedComp.v
@@ -1,25 +1,27 @@
 Require Import Common Monads.
 Require Import Metadata.
-Require ElimFunc2 Switched String.
+Require Import ListLemmas.
+Require ElimFunc2 ElimFunc3 Switched String.
 Delimit Scope string_scope with string.
 
-Module E := ElimFunc2.
-Module S := Switched.
+Module A := ElimFunc3.
+Module AS := ElimFunc2.
+Module B := Switched.
 
 
 Definition unroll_case rec e info :=
-    let fix go n e (info : E.rec_info) :=
+    let fix go n e (info : AS.rec_info) :=
         match info with
         | [] => e
         | r :: info' =>
                 let e' := if r
-                    then S.Call (S.Call e (S.Deref S.Arg n)) (S.Call rec (S.Deref S.Arg n))
-                    else S.Call e (S.Deref S.Arg n) in
+                    then B.Call (B.Call e (B.Deref B.Arg n)) (B.Call rec (B.Deref B.Arg n))
+                    else B.Call e (B.Deref B.Arg n) in
                 go (S n) e' info'
         end in
     go 0 e info.
 
-Definition compile (e : E.expr) : S.expr :=
+Definition compile (e : AS.expr) : B.expr :=
     let fix go e :=
         let fix go_list es :=
             match es with
@@ -27,20 +29,20 @@ Definition compile (e : E.expr) : S.expr :=
             | e :: es => go e :: go_list es
             end in
         match e with
-        | E.Arg => S.Arg
-        | E.UpVar n => S.UpVar n
-        | E.Call f a => S.Call (go f) (go a)
-        | E.Constr tag args => S.Constr tag (go_list args)
-        | E.ElimBody rec cases =>
+        | AS.Arg => B.Arg
+        | AS.UpVar n => B.UpVar n
+        | AS.Call f a => B.Call (go f) (go a)
+        | AS.Constr tag args => B.Constr tag (go_list args)
+        | AS.ElimBody rec cases =>
                 let rec' := go rec in
-                let fix go_cases cases :=
+                let fix go_cases rec' cases :=
                     match cases with
                     | [] => []
                     | (e, info) :: cases =>
-                            unroll_case rec' (go e) info :: go_cases cases
+                            unroll_case rec' (go e) info :: go_cases rec' cases
                     end in
-                S.Switch (go_cases cases) S.Arg
-        | E.Close fname free => S.Close fname (go_list free)
+                B.Switch (go_cases rec' cases)
+        | AS.Close fname free => B.Close fname (go_list free)
         end in go e.
 
 Definition compile_list :=
@@ -51,7 +53,292 @@ Definition compile_list :=
         | e :: es => go e :: go_list es
         end in go_list.
 
-Definition compile_cu (cu : list E.expr * list metadata) : list S.expr * list metadata :=
+Definition compile_cases :=
+    let go := compile in
+    let fix go_cases rec' cases :=
+        match cases with
+        | [] => []
+        | (e, info) :: cases =>
+                unroll_case rec' (go e) info :: go_cases rec' cases
+        end in go_cases.
+
+Ltac refold_compile :=
+    fold compile_list in *;
+    fold compile_cases in *.
+
+Definition compile_cu (cu : list AS.expr * list metadata) : list B.expr * list metadata :=
     let '(exprs, metas) := cu in
     let exprs' := compile_list exprs in
     (exprs', metas).
+
+
+
+Lemma compile_list_is_map : forall es,
+    compile_list es = map compile es.
+induction es; simpl; eauto.
+Qed.
+
+Lemma compile_list_length : forall es,
+    length (compile_list es) = length es.
+induction es; simpl; eauto.
+Qed.
+
+Lemma compile_cases_is_map : forall rec' cases,
+    compile_cases rec' cases =
+        map (fun p => unroll_case rec' (compile (fst p)) (snd p)) cases.
+induction cases; simpl; eauto.
+destruct a. simpl. f_equal. eauto.
+Qed.
+
+
+
+Fixpoint upvar_list' acc n :=
+    match n with
+    | 0 => B.UpVar 0 :: acc
+    | S n' => upvar_list' (B.UpVar n' :: acc) n'
+    end.
+
+Definition upvar_list n := upvar_list' [] n.
+
+
+
+
+Definition I_case (P : AS.expr -> B.expr -> Prop) brec ap bcase :=
+    (* Using `let '(acase, ainfo) := ap` causes the positivity check to fail (???) *)
+    let acase := fst ap in
+    let ainfo := snd ap in
+    exists bcase0,
+        P acase bcase0 /\
+        bcase = unroll_case brec bcase0 ainfo.
+
+Inductive I_expr (AE : AS.env) (BE : B.env) : AS.expr -> B.expr -> Prop :=
+| IArg : I_expr AE BE AS.Arg B.Arg
+| IUpVar : forall n, I_expr AE BE (AS.UpVar n) (B.UpVar n)
+| ICall : forall af aa bf ba,
+        I_expr AE BE af bf ->
+        I_expr AE BE aa ba ->
+        I_expr AE BE (AS.Call af aa) (B.Call bf ba)
+| IConstr :forall tag aargs bargs,
+        Forall2 (I_expr AE BE) aargs bargs ->
+        I_expr AE BE (AS.Constr tag aargs) (B.Constr tag bargs)
+| IElimBody : forall arec acases brec bcases,
+        I_expr AE BE arec brec ->
+        Forall2 (I_case (I_expr AE BE) brec) acases bcases ->
+        I_expr AE BE (AS.ElimBody arec acases) (B.Switch bcases)
+| IClose :forall tag afree bfree,
+        Forall2 (I_expr AE BE) afree bfree ->
+        I_expr AE BE (AS.Close tag afree) (B.Close tag bfree)
+.
+
+Inductive I (AE : AS.env) (BE : B.env) : A.state -> B.state -> Prop :=
+| IRun : forall ae al ak be bl bk,
+        I_expr AE BE ae be ->
+        Forall AS.value al ->
+        Forall B.value bl ->
+        Forall2 (I_expr AE BE) al bl ->
+        (forall av bv,
+            AS.value av ->
+            B.value bv ->
+            I_expr AE BE av bv ->
+            I AE BE (ak av) (bk bv)) ->
+        I AE BE (A.Run ae al ak) (B.Run be bl bk)
+
+| IElimRecVal : forall fname n afree acases al ak bcases bl bk,
+        n = length afree ->
+        afree = skipn 1 (firstn n al) ->
+        Forall2 (I_case (I_expr AE BE) (B.Close fname (upvar_list n))) acases bcases ->
+        Forall AS.value al ->
+        Forall B.value bl ->
+        Forall2 (I_expr AE BE) al bl ->
+        (forall av bv,
+            AS.value av ->
+            B.value bv ->
+            I_expr AE BE av bv ->
+            I AE BE (ak av) (bk bv)) ->
+        I AE BE (A.Run (AS.ElimBody (AS.Close fname afree) acases) al ak)
+                (B.Run (B.Switch bcases) bl bk)
+
+| IStop : forall ae be,
+        I_expr AE BE ae be ->
+        I AE BE (A.Stop ae) (B.Stop be).
+
+
+
+
+Lemma Forall2_same : forall A (P : A -> A -> Prop) xs,
+    Forall2 P xs xs <-> Forall (fun x => P x x) xs.
+induction xs; split; intro; try on _, invc; firstorder eauto.
+Qed.
+
+Theorem compile_I_expr : forall AE BE ae be,
+    compile ae = be ->
+    I_expr AE BE ae be.
+intros AE BE.
+induction ae using AS.expr_rect_mut with
+    (Pl := fun aes => forall bes,
+        compile_list aes = bes ->
+        Forall2 (I_expr AE BE) aes bes)
+    (Pp := fun ap => forall be,
+        compile (fst ap) = be ->
+        I_expr AE BE (fst ap) be)
+    (Plp := fun aps => forall bes,
+        compile_list (map fst aps) = bes ->
+        Forall2 (I_expr AE BE) (map fst aps) bes);
+simpl; eauto;
+intros0 Hcomp; simpl in Hcomp; refold_compile; try rewrite <- Hcomp; eauto.
+
+- constructor.
+- constructor.
+- constructor; eauto.
+- constructor; eauto.
+- econstructor; eauto.
+  rewrite compile_cases_is_map. rewrite <- Forall2_map_r.
+  specialize (IHae0 ?? ***). rewrite compile_list_is_map in *.
+  rewrite <- Forall2_map, <- Forall2_map_r in *.  rewrite Forall2_same in *.
+  list_magic_on (cases, tt). destruct cases_i as [acase info].
+  unfold I_case. exists (compile acase). simpl. split; eauto.
+- constructor; eauto.
+Qed.
+
+
+
+Lemma I_expr_value : forall AE BE a b,
+    I_expr AE BE a b ->
+    AS.value a ->
+    B.value b.
+induction a using AS.expr_ind''; intros0 II Aval; invc II; invc Aval.
+- constructor. list_magic_on (args, (bargs, tt)).
+- constructor. list_magic_on (free, (bfree, tt)).
+Qed.
+Hint Resolve I_expr_value.
+
+Lemma I_expr_value' : forall AE BE b a,
+    I_expr AE BE a b ->
+    B.value b ->
+    AS.value a.
+induction b using B.expr_ind'; intros0 II Bval; invc II; invc Bval.
+- constructor. list_magic_on (args, (aargs, tt)).
+- constructor. list_magic_on (free, (afree, tt)).
+Qed.
+
+Lemma I_expr_not_value : forall AE BE a b,
+    I_expr AE BE a b ->
+    ~AS.value a ->
+    ~B.value b.
+intros. intro. fwd eapply I_expr_value'; eauto.
+Qed.
+Hint Resolve I_expr_not_value.
+
+Lemma I_expr_not_value' : forall AE BE a b,
+    I_expr AE BE a b ->
+    ~B.value b ->
+    ~AS.value a.
+intros. intro. fwd eapply I_expr_value; eauto.
+Qed.
+
+
+
+Definition expr_metric e :=
+    match e with
+    | AS.ElimBody (AS.Close _ free) _ =>
+        (* Count the number of non-values left to evaluate *)
+        fold_left (fun sum e => sum + (if AS.value_dec e then 0 else 1)) free 0
+    | _ => 0
+    end.
+
+Definition metric s :=
+    match s with
+    | A.Run e _ _ => expr_metric e
+    | A.Stop _ => 0
+    end.
+
+Theorem I_sim : forall AE BE a a' b,
+    compile_list AE = BE ->
+    I AE BE a b ->
+    A.sstep AE a a' ->
+    exists b',
+        (B.splus BE b b' \/
+         (b' = b /\ metric a' < metric a)) /\
+        I AE BE a' b'.
+
+destruct a as [ae al ak | ae];
+intros0 Henv II Astep; [ | solve [invc Astep] ].
+
+destruct ae; inv Astep; invc II; try on (I_expr _ _ _ _), invc.
+
+- fwd eapply length_nth_error_Some with (ys := bl) as HH;
+    cycle 1; eauto using Forall2_length.
+    destruct HH as [bv ?].
+
+  eexists. split. left. eapply B.SPlusOne, B.SArg; eauto.
+  on _, eapply_; eapply Forall_nth_error + eapply Forall2_nth_error; eassumption.
+
+- fwd eapply length_nth_error_Some with (ys := bl) as HH;
+    cycle 1; eauto using Forall2_length.
+    destruct HH as [bv ?].
+
+  eexists. split. left. eapply B.SPlusOne, B.SUpVar; eauto.
+  on _, eapply_; eapply Forall_nth_error + eapply Forall2_nth_error; eassumption.
+
+- eexists. split. left. eapply B.SPlusOne, B.SCallL; eauto.
+  constructor; eauto.
+  intros. constructor; eauto.
+  constructor; eauto.
+
+- eexists. split. left. eapply B.SPlusOne, B.SCallR; eauto.
+  constructor; eauto.
+  intros. constructor; eauto.
+  constructor; eauto.
+
+- on (I_expr _ _ (AS.Close _ _) _), invc.
+  fwd eapply length_nth_error_Some with (xs := AE) (ys := compile_list AE) as HH;
+    eauto using compile_list_length.
+    destruct HH as [bbody ?].
+  
+  eexists. split. left. eapply B.SPlusOne, B.SMakeCall; eauto.
+    { list_magic_on (free, (bfree, tt)). }
+  constructor; eauto.
+    { eapply compile_I_expr. pattern body, bbody. eapply Forall2_nth_error; try eassumption.
+      rewrite compile_list_is_map. rewrite <- Forall2_map_r.
+      eapply nth_error_Forall2; eauto. intros. congruence. }
+    { constructor; eauto. list_magic_on (free, (bfree, tt)). }
+
+- on _, invc_using Forall2_3part_inv.
+
+  eexists. split. left. eapply B.SPlusOne, B.SConstrStep; eauto.
+    { list_magic_on (vs, (ys1, tt)). }
+  constructor; eauto.
+  intros. constructor; eauto.
+  constructor; eauto using Forall2_app.
+
+- eexists. split. left. eapply B.SPlusOne, B.SConstrDone; eauto.
+    { list_magic_on (args, (bargs, tt)). }
+  on _, eapply_.
+    { constructor. assumption. }
+    { constructor. list_magic_on (args, (bargs, tt)). }
+  constructor; eauto.
+
+- (* SElimStepRec *) admit.
+
+- (* SEliminate *) admit.
+
+- (* special elim handling *) admit. (* need to adjust IElimRecVal *)
+
+- (* special elim handling *) admit. (* need to adjust IElimRecVal *)
+
+- on _, invc_using Forall2_3part_inv.
+
+  eexists. split. left. eapply B.SPlusOne, B.SCloseStep; eauto.
+    { list_magic_on (vs, (ys1, tt)). }
+  constructor; eauto.
+  intros. constructor; eauto.
+  constructor; eauto using Forall2_app.
+
+- eexists. split. left. eapply B.SPlusOne, B.SCloseDone; eauto.
+    { list_magic_on (free, (bfree, tt)). }
+  on _, eapply_.
+    { constructor. assumption. }
+    { constructor. list_magic_on (free, (bfree, tt)). }
+  constructor; eauto.
+
+Admitted.
